src/NLustre/NLCoindToIndexed.v
@@ -17,6 +17,7 @@ From Velus Require Import NLustre.NLSyntax.
 From Velus Require Import NLustre.NLOrdered.
 From Velus Require Import IndexedStreams.
 From Velus Require Import CoindStreams.
+From Velus Require Import CoindToIndexed.
 
 From Velus Require Import CoreExpr.CESemantics.
 From Velus Require Import NLustre.NLIndexedSemantics.
@@ -32,6 +33,7 @@ Module Type NLCOINDTOINDEXED
        (Import Syn     : NLSYNTAX           Ids Op       CESyn)
        (Import IStr    : INDEXEDSTREAMS         Op OpAux)
        (Import CStr    : COINDSTREAMS           Op OpAux)
+       (Import CIStr   : COINDTOINDEXED         Op OpAux           CStr IStr)
        (Import Ord     : NLORDERED          Ids Op       CESyn Syn)
        (CESem          : CESEMANTICS        Ids Op OpAux CESyn     IStr)
        (Indexed        : NLINDEXEDSEMANTICS Ids Op OpAux CESyn Syn IStr Ord CESem)
@@ -41,220 +43,22 @@ Module Type NLCOINDTOINDEXED
 
     Variable G : global.
 
-    (** * BASIC CORRESPONDENCES *)
-
-    (** ** Definitions  *)
-
-    (** Translate a coinductive Stream into an indexed stream.
-        The result stream is the function which associates the [n]th element of
-        the input Stream to each [n].
-     *)
-    Definition tr_Stream {A} (xs: Stream A) : stream A :=
-      fun n => xs # n.
-
-    (** Translate a list of Streams into a stream of list. *)
-    Definition tr_Streams {A} (xss: list (Stream A)) : stream (list A) :=
-      fun n => List.map (fun xs => tr_Stream xs n) xss.
-
-    (** Translate an history from coinductive to indexed world.
-        Every element of the history is translated.
-     *)
-    Definition tr_history (H: history) : CESem.history :=
-      fun n => Env.map (fun xs => tr_Stream xs n) H.
-
-    (** ** Properties  *)
-
-    (** Indexing a translated Stream at [0] is taking the head of the source
-        Stream. *)
-    Lemma tr_Stream_0:
-      forall {A} (xs: Stream A) x,
-        tr_Stream (x ⋅ xs) 0 = x.
-    Proof. reflexivity. Qed.
-
-    (** Indexing a translated Stream at [S n] is indexing the tail of the source
-        Stream at [n]. *)
-    Lemma tr_Stream_S:
-      forall {A} (xs: Stream A) x n,
-        tr_Stream (x ⋅ xs) (S n) = tr_Stream xs n.
-    Proof. reflexivity. Qed.
-
-    (** Another version of the previous lemma.  *)
-    Lemma tr_Stream_tl:
-      forall {A} (xs: Stream A) n,
-        tr_Stream (tl xs) n = tr_Stream xs (S n).
-    Proof. reflexivity. Qed.
-
-    Lemma tr_Stream_const:
-      forall {A} (c: A) n,
-        tr_Stream (Streams.const c) n = c.
-    Proof.
-      induction n; rewrite unfold_Stream at 1; simpl.
-      - now rewrite tr_Stream_0.
-      - now rewrite tr_Stream_S.
-    Qed.
-
-    (** [tr_Stream] is compatible wrt to [EqSt]. *)
-    Add Parametric Morphism A : (@tr_Stream A)
-        with signature @EqSt A ==> eq ==> eq
-          as tr_Stream_morph.
-    Proof.
-      intros xs ys Exs n.
-      revert xs ys Exs; induction n; intros; destruct xs, ys; inv Exs.
-      - rewrite 2 tr_Stream_0; auto.
-      - rewrite 2 tr_Stream_S; auto.
-    Qed.
-
-    Fact tr_Streams_app:
-      forall A (xss yss: list (Stream A)) n,
-        tr_Streams (xss ++ yss) n = tr_Streams xss n ++ tr_Streams yss n.
-    Proof.
-      unfold tr_Streams; intros; rewrite map_app; auto.
-    Qed.
-
-    (** The counterpart of [tr_Stream_tl] for lists of Streams. *)
-    Lemma tr_Streams_tl:
-      forall A (xss: list (Stream A)) n,
-        tr_Streams (List.map (tl (A:=A)) xss) n = tr_Streams xss (S n).
-    Proof.
-      intros; unfold tr_Streams; rewrite map_map; auto.
-    Qed.
-
-    Lemma tr_Streams_hd:
-      forall A (xss: list (Stream A)),
-        tr_Streams xss 0 = List.map (hd (A:=A)) xss.
-    Proof.
-      reflexivity.
-    Qed.
-
-    (** The counterpart of [tr_Stream_tl] for histories. *)
-    Lemma tr_history_tl:
-      forall n H,
-        tr_history H (S n) = tr_history (history_tl H) n.
-    Proof.
-      now repeat setoid_rewrite Env.map_map.
-    Qed.
-
     (** * SEMANTICS CORRESPONDENCE *)
 
     (** ** Variables *)
-
-    Lemma sem_var_impl:
-      forall H x xs,
-      sem_var H x xs ->
-      CESem.sem_var (tr_history H) x (tr_Stream xs).
-    Proof.
-      intros * Find n.
-      unfold CESem.sem_var_instant.
-      inversion_clear Find as [???? Find' E].
-      unfold tr_history, Env.map.
-      rewrite Env.gmapi, Find', E; simpl; auto.
-    Qed.
-    Hint Resolve sem_var_impl.
 
     Corollary sem_vars_impl:
       forall H xs xss,
       Forall2 (sem_var H) xs xss ->
       CESem.sem_vars (tr_history H) xs (tr_Streams xss).
     Proof.
-      unfold CESem.sem_vars, CESem.lift'.
+      unfold CESem.sem_vars, IStr.lift'.
       induction 1 as [|? ? ? ? Find];
         simpl; intro; constructor; auto.
       - apply sem_var_impl; auto.
       - apply IHForall2.
     Qed.
     Hint Resolve sem_vars_impl.
-
-
-    (** ** Semantics of clocks *)
-
-    (** Give an indexed specification for [sem_clock] in the previous style,
-        with added complexity as [sem_clock] depends on [H] and [b].
-        We go by induction on the clock [ck] then by induction on [n] and
-        inversion of the coinductive hypothesis as before. *)
-    Hint Constructors CESem.sem_clock_instant.
-    Lemma sem_clock_index:
-      forall n H b ck bs,
-        sem_clock H b ck bs ->
-        (ck = Cbase
-         /\ tr_Stream b n = tr_Stream bs n)
-        \/
-        (exists ck' x k c,
-            ck = Con ck' x k
-            /\ CESem.sem_clock_instant
-                (tr_Stream b n) (tr_history H n) ck' true
-            /\ CESem.sem_var_instant (tr_history H n) x
-                                      (present c)
-            /\ val_to_bool c = Some k
-            /\ tr_Stream bs n = true)
-        \/
-        (exists ck' x k,
-            ck = Con ck' x k
-            /\ CESem.sem_clock_instant
-                (tr_Stream b n) (tr_history H n) ck' false
-            /\ CESem.sem_var_instant (tr_history H n) x absent
-            /\ tr_Stream bs n = false)
-        \/
-        (exists ck' x k c,
-            ck = Con ck' x (negb k)
-            /\ CESem.sem_clock_instant
-                (tr_Stream b n) (tr_history H n) ck' true
-            /\ CESem.sem_var_instant (tr_history H n) x
-                                      (present c)
-            /\ val_to_bool c = Some k
-            /\ tr_Stream bs n = false).
-    Proof.
-      Local Ltac rew_0 :=
-        try match goal with
-              H: tr_Stream _ _ = _ |- _ => now rewrite tr_Stream_0 in H
-            end.
-      intros n H b ck; revert n H b; induction ck as [|ck ? x k].
-      - inversion_clear 1 as [? ? ? Eb| | |].
-        left; intuition.
-        now rewrite Eb.
-      - intro n; revert x k; induction n; intros x k H bk bk' Indexed.
-        + inversion_clear Indexed as [|? ? ? ? ? ? ? ? ? IndexedCk Hvar
-                                     |? ? ? ? ? ? ? ? IndexedCk Hvar
-                                     |? ? ? ? ? ? ? ? ? IndexedCk Hvar].
-          * right; left.
-            apply sem_var_impl in Hvar;
-              unfold CESem.sem_var, CESem.lift in Hvar ; specialize (Hvar 0);
-                rewrite tr_Stream_0 in Hvar.
-            do 4 eexists; intuition; eauto.
-            apply (IHck 0) in IndexedCk as [(? & E)|[|[]]]; destruct_conjs;
-              subst; eauto; rew_0.
-            rewrite E, tr_Stream_0; constructor.
-          * right; right; left.
-            apply sem_var_impl in Hvar;
-              unfold CESem.sem_var, CESem.lift in Hvar ; specialize (Hvar 0);
-                rewrite tr_Stream_0 in Hvar.
-            do 3 eexists; intuition.
-            apply (IHck 0) in IndexedCk as [(? & E)|[|[]]]; destruct_conjs;
-              subst; eauto; rew_0.
-            rewrite E, tr_Stream_0; constructor.
-          * right; right; right.
-            apply sem_var_impl in Hvar;
-              unfold CESem.sem_var, CESem.lift in Hvar; specialize (Hvar 0);
-                rewrite tr_Stream_0 in Hvar.
-            do 4 eexists; intuition; eauto.
-            apply (IHck 0) in IndexedCk as [(? & E)|[|[]]]; destruct_conjs;
-              subst; eauto; rew_0.
-            rewrite E, tr_Stream_0; constructor.
-        + inversion_clear Indexed; rewrite <-tr_Stream_tl, tr_history_tl; eauto.
-    Qed.
-
-    (** We can then deduce the correspondence lemma for [sem_clock]. *)
-    Corollary sem_clock_impl:
-      forall H b ck bs,
-        sem_clock H b ck bs ->
-        CESem.sem_clock (tr_Stream b) (tr_history H) ck (tr_Stream bs).
-    Proof.
-      intros * Indexed n.
-      apply (sem_clock_index n) in Indexed. destruct Indexed as [|[|[|]]];
-                                              destruct_conjs;
-        match goal with H: tr_Stream _ _ = _ |- _ => rewrite H end;
-        subst; eauto.
-    Qed.
-    Hint Resolve sem_clock_impl.
 
     (** ** Semantics of exps *)
 
@@ -277,7 +81,7 @@ Module Type NLCOINDTOINDEXED
       - apply sem_var_impl in Hvar; eauto.
       - specialize (IHsem_exp n).
         apply sem_var_impl in Hvar;
-          unfold tr_Stream, CESem.sem_var, CESem.lift in Hvar.
+          unfold tr_Stream, IStr.sem_var, IStr.lift in Hvar.
         specialize (Hvar n); simpl in *.
         rewrite when_spec in Hwhen.
         destruct (Hwhen n)
@@ -315,14 +119,14 @@ Module Type NLCOINDTOINDEXED
     Lemma sem_aexp_index:
       forall n H b ck le es,
         CoInd.sem_aexp H b ck le es ->
-        (CESem.sem_clock_instant (tr_Stream b n)
+        (sem_clock_instant (tr_Stream b n)
                                    (tr_history H n) ck false
          /\ CESem.sem_exp_instant
              (tr_Stream b n) (tr_history H n) le absent
          /\ tr_Stream es n = absent)
         \/
         (exists e,
-            CESem.sem_clock_instant (tr_Stream b n)
+            sem_clock_instant (tr_Stream b n)
                                       (tr_history H n) ck true
             /\ CESem.sem_exp_instant
                 (tr_Stream b n) (tr_history H n) le (present e)
@@ -390,7 +194,7 @@ Module Type NLCOINDTOINDEXED
                     |? ? ? ? He]; intro n.
       - specialize (IHsem_cexp1 n); specialize (IHsem_cexp2 n).
         apply sem_var_impl in Hvar; eauto.
-        unfold tr_Stream, CESem.sem_var, CESem.lift in Hvar.
+        unfold tr_Stream, IStr.sem_var, IStr.lift in Hvar.
         specialize (Hvar n); simpl in *.
         rename H0_ into Hf.
         rewrite merge_spec in Hmerge; destruct (Hmerge n)
@@ -425,14 +229,14 @@ Module Type NLCOINDTOINDEXED
     Lemma sem_caexp_index:
       forall n H b ck le es,
         CoInd.sem_caexp H b ck le es ->
-        (CESem.sem_clock_instant (tr_Stream b n)
+        (sem_clock_instant (tr_Stream b n)
                                    (tr_history H n) ck false
          /\ CESem.sem_cexp_instant
              (tr_Stream b n) (tr_history H n) le absent
          /\ tr_Stream es n = absent)
         \/
         (exists e,
-            CESem.sem_clock_instant (tr_Stream b n)
+            sem_clock_instant (tr_Stream b n)
                                       (tr_history H n) ck true
             /\ CESem.sem_cexp_instant
                 (tr_Stream b n) (tr_history H n) le (present e)
@@ -606,21 +410,21 @@ Module Type NLCOINDTOINDEXED
       intro n; specialize (Var n); specialize (Clock n).
       split; split.
       - intros * Clock'.
-        eapply CESem.sem_clock_instant_det in Clock; eauto.
+        eapply IStr.sem_clock_instant_det in Clock; eauto.
         symmetry in Clock; apply Spec, not_absent_present in Clock as (?& E).
         rewrite E in Var; eauto.
       - intros (?& Var').
-        eapply CESem.sem_var_instant_det in Var; eauto.
+        eapply IStr.sem_var_instant_det in Var; eauto.
         assert (tr_Stream bs n = true) as <-; auto.
         apply Spec; intro; congruence.
       - intros * Clock'.
-        eapply CESem.sem_clock_instant_det in Clock; eauto.
+        eapply IStr.sem_clock_instant_det in Clock; eauto.
         symmetry in Clock; rewrite <-Bool.not_true_iff_false, Spec in Clock.
         assert (tr_Stream xs n = absent) as <-; auto.
         apply Decidable.not_not in Clock; auto.
         apply decidable_eq_value.
       - intros Var'.
-        eapply CESem.sem_var_instant_det in Var; eauto.
+        eapply IStr.sem_var_instant_det in Var; eauto.
         assert (tr_Stream bs n = false) as <-; auto.
         rewrite <-Bool.not_true_iff_false, Spec; auto.
     Qed.
@@ -691,10 +495,11 @@ Module NLCoindToIndexedFun
        (Syn     : NLSYNTAX           Ids Op       CESyn)
        (IStr    : INDEXEDSTREAMS         Op OpAux)
        (CStr    : COINDSTREAMS           Op OpAux)
+       (CIStr   : COINDTOINDEXED         Op OpAux           CStr IStr)
        (Ord     : NLORDERED          Ids Op       CESyn Syn)
        (CESem   : CESEMANTICS        Ids Op OpAux CESyn     IStr)
        (Indexed : NLINDEXEDSEMANTICS Ids Op OpAux CESyn Syn IStr Ord CESem)
        (CoInd   : NLCOINDSEMANTICS   Ids Op OpAux CESyn Syn CStr Ord)
-<: NLCOINDTOINDEXED Ids Op OpAux CESyn Syn IStr CStr Ord CESem Indexed CoInd.
-  Include NLCOINDTOINDEXED Ids Op OpAux CESyn Syn IStr CStr Ord CESem Indexed CoInd.
+<: NLCOINDTOINDEXED Ids Op OpAux CESyn Syn IStr CStr CIStr Ord CESem Indexed CoInd.
+  Include NLCOINDTOINDEXED Ids Op OpAux CESyn Syn IStr CStr CIStr Ord CESem Indexed CoInd.
 End NLCoindToIndexedFun.
