src/NLustre/NLIndexedToCoind.v
@@ -44,107 +44,6 @@ Module Type NLINDEXEDTOCOIND
 
     Variable G : global.
 
-    (** * BASIC CORRESPONDENCES *)
-
-    (** ** Definitions  *)
-
-    (** A generic function to build a coinductive Stream. *)
-    CoFixpoint init_from {A} (n: nat) (f: nat -> A) : Stream A :=
-      f n ⋅ init_from (S n) f.
-
-    (** Translate an indexed stream into a coinductive Stream.
-        The [n]th element of the result Stream is the result of the application
-        of the input stream on [n]. *)
-    Definition tr_stream_from {A} (n: nat) (xs: stream A) : Stream A :=
-      init_from n xs.
-
-    Definition tr_stream {A} : stream A -> Stream A := tr_stream_from 0.
-
-    (** Build a list of coinductive streams from an the integer range [0..m]. *)
-    Definition seq_streams {A} (f: nat -> Stream A) (m: nat) : list (Stream A) :=
-      List.map f (seq 0 m).
-
-    (** Build the indexed stream corresponding to the [i]th elements of
-        the input stream of lists. *)
-    Definition streams_nth (k: nat) (xss: stream (list value)): stream value :=
-      fun n => nth k (xss n) absent.
-
-    (** Build a coinductive Stream extracting the [i]th element of the list
-        obtained at each instant [n]. *)
-    Definition nth_tr_streams_from (n: nat) (xss: stream (list value)) (k: nat)
-      : Stream value :=
-      tr_stream_from n (streams_nth k xss).
-
-    (** Translate an indexed stream of list into a list of coinductive Streams
-        using the two previous functions. *)
-    Definition tr_streams_from (n: nat) (xss: stream (list value))
-      : list (Stream value) :=
-      seq_streams (nth_tr_streams_from n xss) (length (xss n)).
-
-    Definition tr_streams: stream (list value) -> list (Stream value) :=
-      tr_streams_from 0.
-
-    Ltac unfold_tr_streams :=
-      unfold tr_streams, tr_streams_from.
-
-    (** Translate an history from indexed to coinductive world.
-        Every element of the history is translated. *)
-    Definition tr_history_from (n: nat) (H: CESem.history) : history :=
-      Env.mapi (fun x _ => init_from n (fun n => match Env.find x (H n) with
-                                                 | Some v => v
-                                                 | None => absent
-                                                 end)) (H 0).
-
-    Definition tr_history : CESem.history -> history :=
-      tr_history_from 0.
-
-    (** ** Properties  *)
-
-    (** A basic definition-rewriting lemma.  *)
-    Lemma init_from_n:
-      forall {A} (f: nat -> A) n,
-        init_from n f = f n ⋅ init_from (S n) f.
-    Proof.
-      intros; now rewrite unfold_Stream at 1.
-    Qed.
-
-    (** [init_from] is compatible wrt to extensional equality. *)
-    Add Parametric Morphism A : (@init_from A)
-        with signature eq ==> eq_str ==> @EqSt A
-          as init_from_morph.
-    Proof.
-      cofix Cofix. intros x xs xs' E.
-      rewrite init_from_n; rewrite (init_from_n xs').
-      constructor; simpl; auto.
-    Qed.
-
-    (** The [m]th element of the built stream, starting from [n],
-        is the result of the application of [f] at [(m+n)]. *)
-    Lemma init_from_nth:
-      forall {A} m n (f: nat -> A),
-        (init_from n f) # m = f (m + n).
-    Proof.
-      unfold Str_nth; induction m; intros; simpl; auto.
-      now rewrite IHm, <-plus_n_Sm.
-    Qed.
-
-    (** Taking the tail of a built Stream from [n] is building it from [S n]. *)
-    Lemma init_from_tl:
-      forall {A} n (f: nat -> A),
-        tl (init_from n f) = init_from (S n) f.
-    Proof.
-      intros; rewrite init_from_n; auto.
-    Qed.
-
-    (** A generalization for multiple tails. *)
-    Lemma init_from_nth_tl:
-      forall {A} n m (f: nat -> A),
-        Str_nth_tl n (init_from m f) = init_from (n + m) f.
-    Proof.
-      induction n; intros; simpl; auto.
-      now rewrite IHn, Nat.add_succ_r.
-    Qed.
-
     (** The length of the range-built list of Streams is simply the difference
         between the bounds of the range.  *)
     Lemma seq_streams_length:
@@ -202,14 +101,6 @@ Module Type NLINDEXEDTOCOIND
     Proof.
       unfold_tr_streams; intros.
       rewrite seq_streams_length; simpl; omega.
-    Qed.
-
-    (** The counterpart of [tr_stream_from_tl] for histories. *)
-    Lemma tr_history_from_tl:
-      forall n H,
-        history_tl (tr_history_from n H) = tr_history_from (S n) H.
-    Proof.
-      now setoid_rewrite Env.mapi_mapi.
     Qed.
 
     (** If at instant [n], a property is true for all elements of the list
@@ -279,28 +170,6 @@ Module Type NLINDEXEDTOCOIND
     (*     now setoid_rewrite E in Sem. *)
     (* Qed. *)
 
-    Lemma sem_var_impl_from:
-      forall n H x xs,
-        CESem.sem_var H x xs ->
-        CoInd.sem_var (tr_history_from n H) x (tr_stream_from n xs).
-    Proof.
-      unfold CESem.sem_var, CESem.lift', CESem.sem_var_instant.
-      intros * Sem.
-      econstructor.
-      - setoid_rewrite Env.gmapi.
-        rewrite Sem; simpl; eauto.
-      - unfold tr_stream_from.
-        apply ntheq_eqst; intro.
-        now rewrite 2 init_from_nth, Sem.
-    Qed.
-
-    Corollary sem_var_impl:
-      forall H x xs,
-        CESem.sem_var H x xs ->
-        CoInd.sem_var (tr_history H) x (tr_stream xs).
-    Proof. apply sem_var_impl_from. Qed.
-    Hint Resolve sem_var_impl_from sem_var_impl.
-
     (** An inversion principle for [sem_vars]. *)
     Lemma sem_vars_inv_from:
       forall H xs xss,
@@ -337,7 +206,7 @@ Module Type NLINDEXEDTOCOIND
     Corollary sem_vars_impl_from:
       forall n H xs xss,
       CESem.sem_vars H xs xss ->
-      Forall2 (CoInd.sem_var (tr_history_from n H)) xs (tr_streams_from n xss).
+      Forall2 (sem_var (tr_history_from n H)) xs (tr_streams_from n xss).
     Proof.
       intros * Sem.
       assert (length xs = length (xss n)) as Length by
@@ -361,7 +230,7 @@ Module Type NLINDEXEDTOCOIND
     Corollary sem_vars_impl:
       forall H xs xss,
       CESem.sem_vars H xs xss ->
-      Forall2 (CoInd.sem_var (tr_history H)) xs (tr_streams xss).
+      Forall2 (sem_var (tr_history H)) xs (tr_streams xss).
     Proof. apply sem_vars_impl_from. Qed.
     Hint Resolve sem_vars_impl_from sem_vars_impl.
 
@@ -486,85 +355,6 @@ Module Type NLINDEXEDTOCOIND
       - left; exists c1, c2, c'; repeat split; auto; intuition CESem.sem_det.
       - right; repeat split; auto; intuition CESem.sem_det.
     Qed.
-
-    (** An inversion principle for [sem_clock] which also uses the interpretor. *)
-    Lemma sem_clock_inv:
-      forall H b bs ck x k,
-        CESem.sem_clock b H (Con ck x k) bs ->
-        exists bs' xs,
-          CESem.sem_clock b H ck bs'
-          /\ CESem.sem_var H x xs
-          /\
-          (forall n,
-              (exists c,
-                  bs' n = true
-                  /\ xs n = present c
-                  /\ val_to_bool c = Some k
-                  /\ bs n = true)
-              \/
-              (bs' n = false
-               /\ xs n = absent
-               /\ bs n = false)
-              \/
-              (exists c,
-                  bs' n = true
-                  /\ xs n = present c
-                  /\ val_to_bool c = Some (negb k)
-                  /\ bs n = false)
-          ).
-    Proof.
-      intros * Sem.
-      interp_str b H ck Sem.
-      interp_str b H x Sem.
-      do 2 eexists; intuition; eauto.
-      specialize (Sem_ck n); specialize (Sem_x n); specialize (Sem n); inv Sem.
-      - left; exists c; repeat split; auto; intuition CESem.sem_det.
-      - right; left; repeat split; auto; intuition CESem.sem_det.
-      - right; right; exists c; intuition; try CESem.sem_det.
-        now rewrite Bool.negb_involutive.
-    Qed.
-
-    (** We can then deduce the correspondence lemma for [sem_clock].
-        We go by induction on the clock [ck] then we use the above inversion
-        lemma. *)
-    Corollary sem_clock_impl_from:
-      forall H b ck bs,
-        CESem.sem_clock b H ck bs ->
-        forall n, CoInd.sem_clock (tr_history_from n H) (tr_stream_from n b) ck
-                             (tr_stream_from n bs).
-    Proof.
-      induction ck; intros * Sem n.
-      - constructor.
-        revert Sem n; cofix CoFix; intros.
-        rewrite init_from_n; rewrite (init_from_n bs).
-        constructor; simpl; auto.
-        specialize (Sem n); now inv Sem.
-      - apply sem_clock_inv in Sem as (bs' & xs & Sem_bs' & Sem_xs & Spec).
-        revert Spec n; cofix CoFix; intros.
-        rewrite (init_from_n bs).
-        apply IHck with (n:=n) in Sem_bs';
-          rewrite (init_from_n bs') in Sem_bs'.
-        apply (sem_var_impl_from n) in Sem_xs;
-          rewrite (init_from_n xs) in Sem_xs.
-        destruct (Spec n) as [|[]]; destruct_conjs;
-        repeat match goal with H:_ n = _ |- _ => rewrite H in *; clear H end.
-        + econstructor; eauto.
-          rewrite init_from_tl, tr_history_from_tl; auto.
-        + econstructor; eauto.
-          rewrite init_from_tl, tr_history_from_tl; auto.
-        + rewrite <-(Bool.negb_involutive b0).
-          eapply CoInd.Son_abs2; eauto.
-          rewrite init_from_tl, tr_history_from_tl; auto.
-          rewrite Bool.negb_involutive; auto.
-    Qed.
-    Hint Resolve sem_clock_impl_from.
-
-    Corollary sem_clock_impl:
-      forall H b ck bs,
-        CESem.sem_clock b H ck bs ->
-        CoInd.sem_clock (tr_history H) (tr_stream b) ck (tr_stream bs).
-    Proof. intros; apply sem_clock_impl_from; auto. Qed.
-    Hint Resolve sem_clock_impl.
 
     (** ** Semantics of exps *)
 
