src/CoindToIndexed.v
@@ -1,0 +1,232 @@
+From Coq Require Import List.
+Import List.ListNotations.
+Open Scope list_scope.
+From Coq Require Import Setoid.
+From Coq Require Import Morphisms.
+From Coq Require Import NPeano.
+From Coq Require Import Omega.
+From Coq Require Import Program.Tactics.
+
+From Velus Require Import Common.
+From Velus Require Import Environment.
+From Velus Require Import Operators.
+From Velus Require Import IndexedStreams.
+From Velus Require Import CoindStreams.
+
+Module Type COINDTOINDEXED
+       (Import Op    : OPERATORS)
+       (Import OpAux : OPERATORS_AUX Op)
+       (Import CStr  : COINDSTREAMS Op OpAux)
+       (Import IStr  : INDEXEDSTREAMS Op OpAux).
+
+    (** * BASIC CORRESPONDENCES *)
+
+    (** ** Definitions  *)
+
+    (** Translate a coinductive Stream into an indexed stream.
+        The result stream is the function which associates the [n]th element of
+        the input Stream to each [n].
+     *)
+    Definition tr_Stream {A} (xs: Stream A) : stream A :=
+      fun n => xs # n.
+
+    (** Translate a list of Streams into a stream of list. *)
+    Definition tr_Streams {A} (xss: list (Stream A)) : stream (list A) :=
+      fun n => List.map (fun xs => tr_Stream xs n) xss.
+
+    (** Translate an history from coinductive to indexed world.
+        Every element of the history is translated.
+     *)
+    Definition tr_history (H: CStr.history) : history :=
+      fun n => Env.map (fun xs => tr_Stream xs n) H.
+
+    (** ** Properties  *)
+
+    (** Indexing a translated Stream at [0] is taking the head of the source
+        Stream. *)
+    Lemma tr_Stream_0:
+      forall {A} (xs: Stream A) x,
+        tr_Stream (x ⋅ xs) 0 = x.
+    Proof. reflexivity. Qed.
+
+    (** Indexing a translated Stream at [S n] is indexing the tail of the source
+        Stream at [n]. *)
+    Lemma tr_Stream_S:
+      forall {A} (xs: Stream A) x n,
+        tr_Stream (x ⋅ xs) (S n) = tr_Stream xs n.
+    Proof. reflexivity. Qed.
+
+    (** Another version of the previous lemma.  *)
+    Lemma tr_Stream_tl:
+      forall {A} (xs: Stream A) n,
+        tr_Stream (tl xs) n = tr_Stream xs (S n).
+    Proof. reflexivity. Qed.
+
+    Lemma tr_Stream_const:
+      forall {A} (c: A) n,
+        tr_Stream (Streams.const c) n = c.
+    Proof.
+      induction n; rewrite unfold_Stream at 1; simpl.
+      - now rewrite tr_Stream_0.
+      - now rewrite tr_Stream_S.
+    Qed.
+
+    (** [tr_Stream] is compatible wrt to [EqSt]. *)
+    Add Parametric Morphism A : (@tr_Stream A)
+        with signature @EqSt A ==> eq ==> eq
+          as tr_Stream_morph.
+    Proof.
+      intros xs ys Exs n.
+      revert xs ys Exs; induction n; intros; destruct xs, ys; inv Exs.
+      - rewrite 2 tr_Stream_0; auto.
+      - rewrite 2 tr_Stream_S; auto.
+    Qed.
+
+    Fact tr_Streams_app:
+      forall A (xss yss: list (Stream A)) n,
+        tr_Streams (xss ++ yss) n = tr_Streams xss n ++ tr_Streams yss n.
+    Proof.
+      unfold tr_Streams; intros; rewrite map_app; auto.
+    Qed.
+
+    (** The counterpart of [tr_Stream_tl] for lists of Streams. *)
+    Lemma tr_Streams_tl:
+      forall A (xss: list (Stream A)) n,
+        tr_Streams (List.map (tl (A:=A)) xss) n = tr_Streams xss (S n).
+    Proof.
+      intros; unfold tr_Streams; rewrite map_map; auto.
+    Qed.
+
+    Lemma tr_Streams_hd:
+      forall A (xss: list (Stream A)),
+        tr_Streams xss 0 = List.map (hd (A:=A)) xss.
+    Proof.
+      reflexivity.
+    Qed.
+
+    (** The counterpart of [tr_Stream_tl] for histories. *)
+    Lemma tr_history_tl:
+      forall n H,
+        tr_history H (S n) = tr_history (history_tl H) n.
+    Proof.
+      now repeat setoid_rewrite Env.map_map.
+    Qed.
+
+    (** * SEMANTICS CORRESPONDENCE *)
+
+    (** ** Variables *)
+
+    Lemma sem_var_impl:
+      forall H x xs,
+      CStr.sem_var H x xs ->
+      sem_var (tr_history H) x (tr_Stream xs).
+    Proof.
+      intros * Find n.
+      unfold sem_var_instant.
+      inversion_clear Find as [???? Find' E].
+      unfold tr_history, Env.map.
+      rewrite Env.gmapi, Find', E; simpl; auto.
+    Qed.
+    Hint Resolve sem_var_impl.
+
+    (** ** Semantics of clocks *)
+
+    (** Give an indexed specification for [sem_clock] in the previous style,
+        with added complexity as [sem_clock] depends on [H] and [b].
+        We go by induction on the clock [ck] then by induction on [n] and
+        inversion of the coinductive hypothesis as before. *)
+    Hint Constructors sem_clock_instant.
+    Lemma sem_clock_index:
+      forall n H b ck bs,
+        CStr.sem_clock H b ck bs ->
+        (ck = Cbase
+         /\ tr_Stream b n = tr_Stream bs n)
+        \/
+        (exists ck' x k c,
+            ck = Con ck' x k
+            /\ sem_clock_instant
+                (tr_Stream b n) (tr_history H n) ck' true
+            /\ sem_var_instant (tr_history H n) x
+                                      (present c)
+            /\ val_to_bool c = Some k
+            /\ tr_Stream bs n = true)
+        \/
+        (exists ck' x k,
+            ck = Con ck' x k
+            /\ sem_clock_instant
+                (tr_Stream b n) (tr_history H n) ck' false
+            /\ sem_var_instant (tr_history H n) x absent
+            /\ tr_Stream bs n = false)
+        \/
+        (exists ck' x k c,
+            ck = Con ck' x (negb k)
+            /\ sem_clock_instant
+                (tr_Stream b n) (tr_history H n) ck' true
+            /\ sem_var_instant (tr_history H n) x
+                                      (present c)
+            /\ val_to_bool c = Some k
+            /\ tr_Stream bs n = false).
+    Proof.
+      Local Ltac rew_0 :=
+        try match goal with
+              H: tr_Stream _ _ = _ |- _ => now rewrite tr_Stream_0 in H
+            end.
+      intros n H b ck; revert n H b; induction ck as [|ck ? x k].
+      - inversion_clear 1 as [? ? ? Eb| | |].
+        left; intuition.
+        now rewrite Eb.
+      - intro n; revert x k; induction n; intros x k H bk bk' Indexed.
+        + inversion_clear Indexed as [|? ? ? ? ? ? ? ? ? IndexedCk Hvar
+                                     |? ? ? ? ? ? ? ? IndexedCk Hvar
+                                     |? ? ? ? ? ? ? ? ? IndexedCk Hvar].
+          * right; left.
+            apply sem_var_impl in Hvar;
+              unfold IStr.sem_var, IStr.lift in Hvar ; specialize (Hvar 0);
+                rewrite tr_Stream_0 in Hvar.
+            do 4 eexists; intuition; eauto.
+            apply (IHck 0) in IndexedCk as [(? & E)|[|[]]]; destruct_conjs;
+              subst; eauto; rew_0.
+            rewrite E, tr_Stream_0; constructor.
+          * right; right; left.
+            apply sem_var_impl in Hvar;
+              unfold IStr.sem_var, IStr.lift in Hvar ; specialize (Hvar 0);
+                rewrite tr_Stream_0 in Hvar.
+            do 3 eexists; intuition.
+            apply (IHck 0) in IndexedCk as [(? & E)|[|[]]]; destruct_conjs;
+              subst; eauto; rew_0.
+            rewrite E, tr_Stream_0; constructor.
+          * right; right; right.
+            apply sem_var_impl in Hvar;
+              unfold IStr.sem_var, IStr.lift in Hvar; specialize (Hvar 0);
+                rewrite tr_Stream_0 in Hvar.
+            do 4 eexists; intuition; eauto.
+            apply (IHck 0) in IndexedCk as [(? & E)|[|[]]]; destruct_conjs;
+              subst; eauto; rew_0.
+            rewrite E, tr_Stream_0; constructor.
+        + inversion_clear Indexed; rewrite <-tr_Stream_tl, tr_history_tl; eauto.
+    Qed.
+
+    (** We can then deduce the correspondence lemma for [sem_clock]. *)
+    Corollary sem_clock_impl:
+      forall H b ck bs,
+        CStr.sem_clock H b ck bs ->
+        sem_clock (tr_Stream b) (tr_history H) ck (tr_Stream bs).
+    Proof.
+      intros * Indexed n.
+      apply (sem_clock_index n) in Indexed. destruct Indexed as [|[|[|]]];
+                                              destruct_conjs;
+        match goal with H: tr_Stream _ _ = _ |- _ => rewrite H end;
+        subst; eauto.
+    Qed.
+    Hint Resolve sem_clock_impl.
+
+End COINDTOINDEXED.
+
+Module CoindToIndexedFun
+       (Op      : OPERATORS)
+       (OpAux   : OPERATORS_AUX          Op)
+       (CStr    : COINDSTREAMS           Op OpAux)
+       (IStr    : INDEXEDSTREAMS         Op OpAux)
+<: COINDTOINDEXED Op OpAux CStr IStr.
+  Include COINDTOINDEXED Op OpAux CStr IStr.
+End CoindToIndexedFun.
