src/IndexedToCoind.v
@@ -1,0 +1,265 @@
+From Coq Require Import List.
+Import List.ListNotations.
+Open Scope list_scope.
+From Coq Require Import Setoid.
+From Coq Require Import Morphisms.
+From Coq Require Import NPeano.
+From Coq Require Import Omega.
+From Coq Require Import Program.Tactics.
+
+From Velus Require Import Common.
+From Velus Require Import Environment.
+From Velus Require Import Operators.
+From Velus Require Import IndexedStreams.
+From Velus Require Import CoindStreams.
+
+Module Type INDEXEDTOCOIND
+       (Import Op    : OPERATORS)
+       (Import OpAux : OPERATORS_AUX Op)
+       (Import IStr  : INDEXEDSTREAMS Op OpAux)
+       (Import CStr  : COINDSTREAMS Op OpAux).
+
+  (** * BASIC CORRESPONDENCES *)
+
+  (** ** Definitions  *)
+
+  (** A generic function to build a coinductive Stream. *)
+  CoFixpoint init_from {A} (n: nat) (f: nat -> A) : Stream A :=
+    f n ⋅ init_from (S n) f.
+
+  (** Translate an indexed stream into a coinductive Stream.
+        The [n]th element of the result Stream is the result of the application
+        of the input stream on [n]. *)
+  Definition tr_stream_from {A} (n: nat) (xs: stream A) : Stream A :=
+    init_from n xs.
+
+  Definition tr_stream {A} : stream A -> Stream A := tr_stream_from 0.
+
+  (** Build a list of coinductive streams from an the integer range [0..m]. *)
+  Definition seq_streams {A} (f: nat -> Stream A) (m: nat) : list (Stream A) :=
+    List.map f (seq 0 m).
+
+  (** Build the indexed stream corresponding to the [i]th elements of
+        the input stream of lists. *)
+  Definition streams_nth (k: nat) (xss: stream (list value)): stream value :=
+    fun n => nth k (xss n) absent.
+
+  (** Build a coinductive Stream extracting the [i]th element of the list
+        obtained at each instant [n]. *)
+  Definition nth_tr_streams_from (n: nat) (xss: stream (list value)) (k: nat)
+    : Stream value :=
+    tr_stream_from n (streams_nth k xss).
+
+  (** Translate an indexed stream of list into a list of coinductive Streams
+        using the two previous functions. *)
+  Definition tr_streams_from (n: nat) (xss: stream (list value))
+    : list (Stream value) :=
+    seq_streams (nth_tr_streams_from n xss) (length (xss n)).
+
+  Definition tr_streams: stream (list value) -> list (Stream value) :=
+    tr_streams_from 0.
+
+  Ltac unfold_tr_streams :=
+    unfold tr_streams, tr_streams_from.
+
+  (** Translate an history from indexed to coinductive world.
+        Every element of the history is translated. *)
+  Definition tr_history_from (n: nat) (H: IStr.history) : history :=
+    Env.mapi (fun x _ => init_from n (fun n => match Env.find x (H n) with
+                                         | Some v => v
+                                         | None => absent
+                                         end)) (H 0).
+
+
+  (** Translate an history from coinductive to indexed world.
+      Every element of the history is translated.
+   *)
+  Definition tr_history : IStr.history -> history :=
+    tr_history_from 0.
+
+  (** The counterpart of [tr_stream_from_tl] for histories. *)
+  Lemma tr_history_from_tl:
+    forall n H,
+      history_tl (tr_history_from n H) = tr_history_from (S n) H.
+  Proof.
+    now setoid_rewrite Env.mapi_mapi.
+  Qed.
+
+  (** ** Properties  *)
+
+  (** A basic definition-rewriting lemma.  *)
+  Lemma init_from_n:
+    forall {A} (f: nat -> A) n,
+      init_from n f = f n ⋅ init_from (S n) f.
+  Proof.
+    intros; now rewrite unfold_Stream at 1.
+  Qed.
+
+  (** [init_from] is compatible wrt to extensional equality. *)
+  Add Parametric Morphism A : (@init_from A)
+      with signature eq ==> eq_str ==> @EqSt A
+        as init_from_morph.
+  Proof.
+    cofix Cofix. intros x xs xs' E.
+    rewrite init_from_n; rewrite (init_from_n xs').
+    constructor; simpl; auto.
+  Qed.
+
+  (** The [m]th element of the built stream, starting from [n],
+        is the result of the application of [f] at [(m+n)]. *)
+  Lemma init_from_nth:
+    forall {A} m n (f: nat -> A),
+      (init_from n f) # m = f (m + n).
+  Proof.
+    unfold Str_nth; induction m; intros; simpl; auto.
+    now rewrite IHm, <-plus_n_Sm.
+  Qed.
+
+  (** Taking the tail of a built Stream from [n] is building it from [S n]. *)
+  Lemma init_from_tl:
+    forall {A} n (f: nat -> A),
+      tl (init_from n f) = init_from (S n) f.
+  Proof.
+    intros; rewrite init_from_n; auto.
+  Qed.
+
+  (** A generalization for multiple tails. *)
+  Lemma init_from_nth_tl:
+    forall {A} n m (f: nat -> A),
+      Str_nth_tl n (init_from m f) = init_from (n + m) f.
+  Proof.
+    induction n; intros; simpl; auto.
+    now rewrite IHn, Nat.add_succ_r.
+  Qed.
+
+  (** * SEMANTICS CORRESPONDENCE *)
+
+  Lemma sem_var_impl_from:
+    forall n H x xs,
+      IStr.sem_var H x xs ->
+      sem_var (tr_history_from n H) x (tr_stream_from n xs).
+  Proof.
+    unfold IStr.sem_var, IStr.lift', sem_var_instant.
+    intros * Sem.
+    econstructor.
+    - unfold Env.MapsTo. setoid_rewrite Env.gmapi.
+      rewrite Sem; simpl; eauto.
+    - unfold tr_stream_from.
+      apply ntheq_eqst; intro.
+      now rewrite 2 init_from_nth, Sem.
+  Qed.
+
+  Corollary sem_var_impl:
+    forall H x xs,
+      IStr.sem_var H x xs ->
+      sem_var (tr_history H) x (tr_stream xs).
+  Proof. apply sem_var_impl_from. Qed.
+  Hint Resolve sem_var_impl_from sem_var_impl.
+
+  (** This tactic automatically uses the interpretor to give a witness stream. *)
+  Ltac interp_str b H x Sem :=
+    let Sem_x := fresh "Sem_" x in
+    let sol sem interp sound :=
+        assert (sem b H x (interp b H x)) as Sem_x
+            by (intro; match goal with n:nat |- _ => specialize (Sem n) end;
+                unfold interp, lift_interp; inv Sem; erewrite <-sound; eauto)
+    in
+    let sol' sem interp sound :=
+        assert (sem H x (interp H x)) as Sem_x
+            by (intro; match goal with n:nat |- _ => specialize (Sem n) end;
+                unfold interp, lift_interp'; inv Sem; erewrite <-sound; eauto)
+    in
+    match type of x with
+    | ident => sol' IStr.sem_var interp_var interp_var_instant_sound
+    | clock => sol IStr.sem_clock interp_clock interp_clock_instant_sound
+    end.
+
+  (** An inversion principle for [sem_clock] which also uses the interpretor. *)
+  Lemma sem_clock_inv:
+    forall H b bs ck x k,
+      IStr.sem_clock b H (Con ck x k) bs ->
+      exists bs' xs,
+        IStr.sem_clock b H ck bs'
+        /\ IStr.sem_var H x xs
+        /\
+        (forall n,
+            (exists c,
+                bs' n = true
+                /\ xs n = present c
+                /\ val_to_bool c = Some k
+                /\ bs n = true)
+            \/
+            (bs' n = false
+             /\ xs n = absent
+             /\ bs n = false)
+            \/
+            (exists c,
+                bs' n = true
+                /\ xs n = present c
+                /\ val_to_bool c = Some (negb k)
+                /\ bs n = false)
+        ).
+  Proof.
+    intros * Sem.
+    interp_str b H ck Sem.
+    interp_str b H x Sem.
+    do 2 eexists; intuition; eauto.
+       specialize (Sem_ck n); specialize (Sem_x n); specialize (Sem n); inv Sem.
+       - left; exists c; repeat split; auto; intuition sem_det.
+       - right; left; repeat split; auto; intuition sem_det.
+       - right; right; exists c; intuition; try sem_det.
+         now rewrite Bool.negb_involutive.
+  Qed.
+
+  (** We can then deduce the correspondence lemma for [sem_clock].
+        We go by induction on the clock [ck] then we use the above inversion
+        lemma. *)
+  Corollary sem_clock_impl_from:
+    forall H b ck bs,
+      IStr.sem_clock b H ck bs ->
+      forall n, sem_clock (tr_history_from n H) (tr_stream_from n b) ck
+                     (tr_stream_from n bs).
+  Proof.
+    induction ck; intros * Sem n.
+    - constructor.
+      revert Sem n; cofix CoFix; intros.
+      rewrite init_from_n; rewrite (init_from_n bs).
+      constructor; simpl; auto.
+      specialize (Sem n); now inv Sem.
+    - apply sem_clock_inv in Sem as (bs' & xs & Sem_bs' & Sem_xs & Spec).
+      revert Spec n; cofix CoFix; intros.
+      rewrite (init_from_n bs).
+      apply IHck with (n:=n) in Sem_bs';
+        rewrite (init_from_n bs') in Sem_bs'.
+      apply (sem_var_impl_from n) in Sem_xs;
+        rewrite (init_from_n xs) in Sem_xs.
+      destruct (Spec n) as [|[]]; destruct_conjs;
+        repeat match goal with H:_ n = _ |- _ => rewrite H in *; clear H end.
+      + econstructor; eauto.
+        rewrite init_from_tl, tr_history_from_tl; auto.
+      + econstructor; eauto.
+        rewrite init_from_tl, tr_history_from_tl; auto.
+      + rewrite <-(Bool.negb_involutive b0).
+        eapply Son_abs2; eauto.
+        rewrite init_from_tl, tr_history_from_tl; auto.
+        rewrite Bool.negb_involutive; auto.
+  Qed.
+  Hint Resolve sem_clock_impl_from.
+
+  Corollary sem_clock_impl:
+    forall H b ck bs,
+      IStr.sem_clock b H ck bs ->
+      sem_clock (tr_history H) (tr_stream b) ck (tr_stream bs).
+  Proof. intros; apply sem_clock_impl_from; auto. Qed.
+  Hint Resolve sem_clock_impl.
+
+End INDEXEDTOCOIND.
+
+Module IndexedToCoindFun
+       (Op      : OPERATORS)
+       (OpAux   : OPERATORS_AUX          Op)
+       (IStr    : INDEXEDSTREAMS         Op OpAux)
+       (CStr    : COINDSTREAMS           Op OpAux)
+<: INDEXEDTOCOIND Op OpAux IStr CStr.
+  Include INDEXEDTOCOIND Op OpAux IStr CStr.
+End IndexedToCoindFun.
