src/Lustre/Lustre.v
@@ -1,6 +1,6 @@
 From Velus Require Import Operators.
 From Velus Require Import Clocks.
-From Velus Require Import CoindStreams.
+From Velus Require Import CoindStreams IndexedStreams.
 From Velus Require Export Lustre.LSyntax.
 From Velus Require Export Lustre.LClocking.
 From Velus Require Export Lustre.LTyping.
@@ -17,29 +17,31 @@ Module Type LUSTRE
        (Ids   : IDS)
        (Op    : OPERATORS)
        (OpAux : OPERATORS_AUX Op)
-       (Str   : COINDSTREAMS  Op OpAux).
+       (CStr  : COINDSTREAMS  Op OpAux)
+       (IStr  : INDEXEDSTREAMS Op OpAux).
   Declare Module Export Syn: LSYNTAX    Ids Op.
   Declare Module Export Typ: LTYPING    Ids Op       Syn.
   Declare Module Export Clo: LCLOCKING  Ids Op       Syn.
   Declare Module Export Ord: LORDERED   Ids Op       Syn.
   Declare Module Export Cau: LCAUSALITY Ids Op       Syn.
-  Declare Module Export Sem: LSEMANTICS Ids Op OpAux Syn Ord Str.
-  Declare Module Export ClSem: LCLOCKSEMANTICS Ids Op OpAux Syn Typ Clo Cau Ord Str Sem.
-  Declare Module Export Norm: LNORMALIZATION Ids Op OpAux Str Syn Typ Clo Cau Ord Sem ClSem.
+  Declare Module Export Sem: LSEMANTICS Ids Op OpAux Syn Ord CStr.
+  Declare Module Export ClSem: LCLOCKSEMANTICS Ids Op OpAux Syn Typ Clo Cau Ord CStr IStr Sem.
+  Declare Module Export Norm: LNORMALIZATION Ids Op OpAux CStr IStr Syn Typ Clo Cau Ord Sem ClSem.
 End LUSTRE.
 
 Module LustreFun
        (Ids   : IDS)
        (Op    : OPERATORS)
        (OpAux : OPERATORS_AUX Op)
-       (Str   : COINDSTREAMS  Op OpAux)
-       <: LUSTRE Ids Op OpAux Str.
+       (CStr  : COINDSTREAMS  Op OpAux)
+       (IStr  : INDEXEDSTREAMS Op OpAux)
+       <: LUSTRE Ids Op OpAux CStr IStr.
   Module Export Syn := LSyntaxFun     Ids Op.
   Module Export Typ := LTypingFun     Ids Op       Syn.
   Module Export Clo := LClockingFun   Ids Op       Syn.
   Module Export Ord:= LOrderedFun     Ids Op       Syn.
   Module Export Cau:= LCausality      Ids Op       Syn.
-  Module Export Sem := LSemanticsFun  Ids Op OpAux Syn Ord Str.
-  Module Export ClSem := LClockSemanticsFun Ids Op OpAux Syn Typ Clo Cau Ord Str Sem.
-  Module Export Norm := LNormalizationFun Ids Op OpAux Str Syn Typ Clo Cau Ord Sem ClSem.
+  Module Export Sem := LSemanticsFun  Ids Op OpAux Syn Ord CStr.
+  Module Export ClSem := LClockSemanticsFun Ids Op OpAux Syn Typ Clo Cau Ord CStr IStr Sem.
+  Module Export Norm := LNormalizationFun Ids Op OpAux CStr IStr Syn Typ Clo Cau Ord Sem ClSem.
 End LustreFun.
