src/Lustre/Normalization/LNormalization.v
@@ -1,6 +1,6 @@
 From Velus Require Import Common Ident.
 From Velus Require Import Operators Environment.
-From Velus Require Import CoindStreams.
+From Velus Require Import CoindStreams IndexedStreams.
 From Velus Require Import Lustre.LSyntax Lustre.LTyping Lustre.LClocking.
 From Velus Require Import Lustre.LCausality Lustre.LOrdered.
 From Velus Require Import Lustre.LSemantics LClockSemantics.
@@ -13,16 +13,17 @@ Module Type LNORMALIZATION
        (Ids : IDS)
        (Op : OPERATORS)
        (OpAux : OPERATORS_AUX Op)
-       (Str : COINDSTREAMS Op OpAux)
+       (CStr : COINDSTREAMS Op OpAux)
+       (IStr : INDEXEDSTREAMS Op OpAux)
        (Syn : LSYNTAX Ids Op)
        (Typ : LTYPING Ids Op Syn)
        (Clo : LCLOCKING Ids Op Syn)
        (Cau : LCAUSALITY Ids Op Syn)
        (Ord : LORDERED Ids Op Syn)
-       (Sem : LSEMANTICS Ids Op OpAux Syn Ord Str)
-       (ClSem : LCLOCKSEMANTICS Ids Op OpAux Syn Typ Clo Cau Ord Str Sem).
+       (Sem : LSEMANTICS Ids Op OpAux Syn Ord CStr)
+       (ClSem : LCLOCKSEMANTICS Ids Op OpAux Syn Typ Clo Cau Ord CStr IStr Sem).
   Declare Module Norm : NORMALIZATION Ids Op OpAux Syn Cau.
-  Declare Module Export Correct : CORRECTNESS Ids Op OpAux Str Syn Cau Typ Clo Ord Sem ClSem Norm.
+  Declare Module Export Correct : CORRECTNESS Ids Op OpAux CStr IStr Syn Cau Typ Clo Ord Sem ClSem Norm.
   Declare Module Idempotence : IDEMPOTENCE Ids Op OpAux Syn Cau Norm.
 End LNORMALIZATION.
 
@@ -30,16 +31,17 @@ Module LNormalizationFun
        (Ids : IDS)
        (Op : OPERATORS)
        (OpAux : OPERATORS_AUX Op)
-       (Str : COINDSTREAMS Op OpAux)
+       (CStr : COINDSTREAMS Op OpAux)
+       (IStr : INDEXEDSTREAMS Op OpAux)
        (Syn : LSYNTAX Ids Op)
        (Typ : LTYPING Ids Op Syn)
        (Clo : LCLOCKING Ids Op Syn)
        (Cau : LCAUSALITY Ids Op Syn)
        (Ord : LORDERED Ids Op Syn)
-       (Sem : LSEMANTICS Ids Op OpAux Syn Ord Str)
-       (ClSem : LCLOCKSEMANTICS Ids Op OpAux Syn Typ Clo Cau Ord Str Sem)
-       <: LNORMALIZATION Ids Op OpAux Str Syn Typ Clo Cau Ord Sem ClSem.
+       (Sem : LSEMANTICS Ids Op OpAux Syn Ord CStr)
+       (ClSem : LCLOCKSEMANTICS Ids Op OpAux Syn Typ Clo Cau Ord CStr IStr Sem)
+       <: LNORMALIZATION Ids Op OpAux CStr IStr Syn Typ Clo Cau Ord Sem ClSem.
   Module Norm := NormalizationFun Ids Op OpAux Syn Cau.
-  Module Export Correct := CorrectnessFun Ids Op OpAux Str Syn Cau Typ Clo Ord Sem ClSem Norm.
+  Module Export Correct := CorrectnessFun Ids Op OpAux CStr IStr Syn Cau Typ Clo Ord Sem ClSem Norm.
   Module Idempotence := IdempotenceFun Ids Op OpAux Syn Cau Norm.
 End LNormalizationFun.
