src/NLustre/NLustre.v
@@ -15,6 +15,7 @@ From Velus Require Export NLustre.NLClockingSemantics.
 From Velus Require Export NLustre.NLTyping.
 From Velus Require Export NLustre.NLNormalArgs.
 From Velus Require Export CoindStreams.
+From Velus Require Import CoindToIndexed.
 
 From Velus Require Import Common.
 
@@ -24,6 +25,7 @@ Module Type NLUSTRE
        (OpAux : OPERATORS_AUX  Op)
        (CStr  : COINDSTREAMS   Op OpAux)
        (IStr  : INDEXEDSTREAMS Op OpAux)
+       (CIStr : COINDTOINDEXED Op OpAux CStr IStr)
        (CE    : COREEXPR Ids   Op OpAux IStr).
   Declare Module Export Syn        : NLSYNTAX             Ids Op       CE.Syn.
   Declare Module Export Ord        : NLORDERED            Ids Op       CE.Syn Syn.
@@ -31,7 +33,7 @@ Module Type NLUSTRE
   Declare Module Export IsF        : ISFREE               Ids Op       CE.Syn Syn CE.IsF.
   Declare Module Export CoindSem   : NLCOINDSEMANTICS     Ids Op OpAux CE.Syn Syn CStr Ord.
   Declare Module Export Sem        : NLINDEXEDSEMANTICS   Ids Op OpAux CE.Syn Syn IStr Ord CE.Sem.
-  Declare Module Export CoindToIdx : NLCOINDTOINDEXED     Ids Op OpAux CE.Syn Syn IStr CStr Ord CE.Sem Sem CoindSem.
+  Declare Module Export CoindToIdx : NLCOINDTOINDEXED     Ids Op OpAux CE.Syn Syn IStr CStr CIStr Ord CE.Sem Sem CoindSem.
   Declare Module Export Typ        : NLTYPING             Ids Op       CE.Syn Syn     Ord CE.Typ.
   Declare Module Export Mem        : MEMORIES             Ids Op       CE.Syn Syn.
   Declare Module Export IsD        : ISDEFINED            Ids Op       CE.Syn Syn                     Mem.
@@ -48,15 +50,16 @@ Module NLustreFun
        (OpAux : OPERATORS_AUX  Op)
        (CStr  : COINDSTREAMS   Op OpAux)
        (IStr  : INDEXEDSTREAMS Op OpAux)
+       (CIStr : COINDTOINDEXED Op OpAux CStr IStr)
        (CE    : COREEXPR Ids   Op OpAux IStr)
-<: NLUSTRE Ids Op OpAux CStr IStr CE.
+<: NLUSTRE Ids Op OpAux CStr IStr CIStr CE.
   Module Export Syn        := NLSyntaxFun             Ids Op       CE.Syn.
   Module Export Ord        := NLOrderedFun            Ids Op       CE.Syn Syn.
   Module Export Norm       := NLNormalArgsFun         Ids Op       CE.Syn Syn.
   Module Export IsF        := IsFreeFun               Ids Op       CE.Syn Syn CE.IsF.
   Module Export CoindSem   := NLCoindSemanticsFun     Ids Op OpAux CE.Syn Syn CStr Ord.
   Module Export Sem        := NLIndexedSemanticsFun   Ids Op OpAux CE.Syn Syn IStr Ord CE.Sem.
-  Module Export CoindToIdx := NLCoindToIndexedFun     Ids Op OpAux CE.Syn Syn IStr CStr Ord CE.Sem Sem CoindSem.
+  Module Export CoindToIdx := NLCoindToIndexedFun     Ids Op OpAux CE.Syn Syn IStr CStr CIStr Ord CE.Sem Sem CoindSem.
   Module Export Typ        := NLTypingFun             Ids Op       CE.Syn Syn     Ord CE.Typ.
   Module Export Mem        := MemoriesFun             Ids Op       CE.Syn Syn.
   Module Export IsD        := IsDefinedFun            Ids Op       CE.Syn Syn                     Mem.
